src/sequential/DelayedStep.v
@@ -1262,3 +1262,84 @@ Module DConfiguration.
     eapply ld_conf_behavior; eauto.
   Qed.
 End DConfiguration.
+
+
+
+Lemma dstep_rtc_all_step lang e th0 th1
+      (STEP: dstep e th0 th1)
+  :
+    rtc (@Thread.all_step lang) th0 th1.
+Proof.
+  inv STEP. etrans.
+  { eapply rtc_implies; [|eapply PROMISES].
+    i. inv H. inv TSTEP. econs; eauto.
+  }
+  etrans.
+  { eapply rtc_implies; [|eapply LOWERS].
+    i. inv H. inv TSTEP. econs; eauto. econs; eauto. econs 2; eauto.
+  }
+  econs 2; [|refl]. econs; eauto. econs; eauto.
+Qed.
+
+Lemma rtc_tau_dstep_rtc_all_step lang th0 th1
+      (STEPS: rtc (tau (@dstep lang)) th0 th1)
+  :
+    rtc (@Thread.all_step lang) th0 th1.
+Proof.
+  induction STEPS.
+  { refl. }
+  etrans; [|eauto]. inv H.
+  eapply dstep_rtc_all_step; eauto.
+Qed.
+
+Lemma dsteps_rtc_all_step lang e th0 th1
+      (STEPS: dsteps e th0 th1)
+  :
+    rtc (@Thread.all_step lang) th0 th1.
+Proof.
+  inv STEPS.
+  { etrans.
+    { eapply rtc_tau_dstep_rtc_all_step; eauto. }
+    { eapply rtc_implies; [|eapply PROMISES].
+      i. inv H. inv TSTEP. econs; eauto.
+    }
+  }
+  { etrans.
+    { eapply rtc_tau_dstep_rtc_all_step; eauto. }
+    { eapply dstep_rtc_all_step; eauto. }
+  }
+Qed.
+
+Lemma delayed_consistent_promise_consistent lang (th: Thread.t lang)
+      (CONSISTENT: delayed_consistent th)
+      (MEM: Memory.closed th.(Thread.memory))
+      (LOCAL: Local.wf th.(Thread.local) th.(Thread.memory))
+      (SC: Memory.closed_timemap th.(Thread.sc) th.(Thread.memory))
+  :
+    Local.promise_consistent th.(Thread.local).
+Proof.
+  hexploit Memory.cap_exists; eauto. i. des.
+  hexploit Local.cap_wf; eauto. i.
+  hexploit Memory.cap_closed_timemap; eauto. i.
+  hexploit Memory.cap_closed; eauto. i.
+  exploit CONSISTENT; eauto. i. des.
+  { pose proof (dsteps_rtc_all_step DSTEPS) as STEPS.
+    eapply rtc_all_step_promise_consistent in STEPS; eauto; ss.
+    inv DSTEPS; ss. inv DSTEP. inv STEP_RELEASE; inv STEP; ss.
+    inv LOCAL0; ss; inv LOCAL1; ss.
+  }
+  { pose proof (dsteps_rtc_all_step DSTEPS) as STEPS.
+    eapply rtc_all_step_promise_consistent in STEPS; eauto; ss.
+    eapply Local.bot_promise_consistent in PROMISES; eauto.
+  }
+Qed.
+
+Lemma DConfiguration_step_future c0 c1 e tid
+      (STEP: DConfiguration.step e tid c0 c1)
+      (WF: Configuration.wf c0)
+  :
+  (<<WF2: Configuration.wf c1>>) /\
+  (<<SC_FUTURE: TimeMap.le (Configuration.sc c0) (Configuration.sc c1)>>) /\
+  (<<MEM_FUTURE: Memory.future (Configuration.memory c0) (Configuration.memory c1)>>).
+Proof.
+Admitted.
